All definitions

QuantifierLean/ExtraParamV3.lean
@@ -6,31 +6,231 @@ import QuantifierLean.Lemmas2_1
 
 open Mathlib
 
-theorem f_inv_on {l a: Vector Int (k+1)} (p: Props2 a n):
+-- @[inline] def Vector.range (n : Nat) : Vector Nat n := ⟨List.range n, by simp⟩
+
+@[inline] def Vector.fin_range (n : Nat) : Vector (Fin n) n :=
+  ⟨(List.range n).pmap (fun i h => ⟨i, h⟩) (by simp), by simp⟩
+
+@[simp]
+lemma Vector.get_fin_range (n: Nat) (i: Fin n): (Vector.fin_range n).get i = i := by
+  simp [Vector.fin_range]
+  rw [Vector.get]
+  simp
+  rw [List.getElem_pmap]
+  simp
+
+def f_inv'' (off: Int) (as ls: Mathlib.Vector Int (k+1)) (x': Int): Vector Int (k+1) :=
+  (Vector.fin_range (k+1)).map fun i => base off as x' i / |as.get i| + ls.get i
+
+lemma f_inv_same (k: Nat) (as ls: Vector Int (k+1)):
+  f_inv'' off as ls x' = f_inv off as ls x' := by
+  rw [f_inv'']
+  apply Mathlib.Vector.ext
+  intro i
+  rw [f_get_is_f_inv_el]
+  simp
+  rw [f_inv_el]
+
+def Fin.FinSet (n: Nat): Finset (Fin n) :=
+  Finset.attachFin (Finset.range n) (by intro m; simp)
+
+def f' (b: Int) (as xs:  Vector Int k) : Int :=
+  b + ∑ i ∈ Fin.FinSet k, as.get i * xs.get i
+
+lemma Multiset.pmap_map {p : β → Prop} (g : ∀ b, p b → γ) (f : α → β) (s) :
+    ∀ H, (pmap g (map f s) H) = pmap (fun a h => g (f a) h) s fun _ h => H _ (mem_map_of_mem _ h):= by
+    induction s using Quot.inductionOn with
+    | h l =>
+      intro H
+      apply congr_arg _ (List.pmap_map g f l H)
+
+lemma fin_sum_prod {k: Nat} (x y: Vector Int k) :
+  ∑ i in Fin.FinSet k, x.get i * y.get i = prodSum x y := by
+  induction k with
+  | zero =>
+    match x, y with
+    | ⟨[],_⟩, ⟨[],_⟩ =>
+    simp [prodSum, Fin.FinSet, Finset.attachFin]
+  | succ k ih =>
+    cases' x, y using Vector.casesOn₂ with cons x y xs ys
+    rw [prodSum_cons]
+    rw [<- ih xs ys]
+    conv =>
+      rw [Fin.FinSet]
+      arg 1; arg 1; arg 1
+      rw [Finset.range]
+      arg 1
+      rw [Nat.add_comm, Multiset.range_add]
+    rw [Finset.sum, Finset.val, Finset.attachFin]
+    simp
+    rw [Multiset.map_pmap, Multiset.pmap_map]
+    -- Rewrite rhs
+    rw[Fin.FinSet, Finset.attachFin, Finset.sum]
+    rw [Multiset.map_pmap]
+    apply congr_arg
+    apply Multiset.pmap_congr
+    intro i _ lt lt2
+    have eq: (⟨1 + i, lt⟩: Fin (k+1)) = (⟨i, lt2⟩: Fin k).succ := by
+      simp
+      rw [Nat.add_comm]
+    rw [eq, Vector.get_cons_succ, Vector.get_cons_succ]
+
+lemma f_equiv (b: Int) (as xs:  Vector Int k):
+  f' b as xs = f b as ls_zero xs := by
+  rw [f', f]
+  rw [fin_sum_prod]
+  simp
+
+
+theorem f_inv_on {a l: Vector Int (k+1)} (p: Props2 a n):
   Set.InvOn (f_inv (offset b a l) a l) (f b a ls_zero) (X2 a l n) (Y2 a (offset b a l) n) := by
   rw [← f_lzero]
   rw [f_comp', f_comp]
   apply f_comp_comp_inv_on p
 
+lemma f_maps_to'{a l: Vector Int (k+1)} (p: Props2 a n): Set.MapsTo (f b a ls_zero) (X2 a l n) (Y2 a (offset b a l) n) := by
+  rw [← @f_lzero k b l]
+  rw [f_comp]
+  have h_m := @h_maps_to (offset b a l) k a n
+  apply Set.MapsTo.comp
+  · apply h_maps_to
+  · apply Set.MapsTo.comp
+    · apply (f_maps_to p)
+    · apply g_maps_to
+
+lemma f_inv_maps_to'{a l: Vector Int (k+1)} (p: Props2 a n): Set.MapsTo (f_inv (offset b a l) a l) (Y2 a (offset b a l) n) (X2 a l n) := by
+  rw [f_comp']
+  apply Set.MapsTo.comp
+  · apply Set.MapsTo.comp
+    · apply g_maps_to'
+    · apply f_inv_maps_to p
+  · apply  h_maps_to'
 
 theorem f_bij_on {l a: Vector Int (k+1)} (p: Props2 a n):
   Set.BijOn (f b a ls_zero) (X2 a l n) (Y2 a (offset b a l) n) := by
-  have hf : Set.MapsTo (f b a ls_zero) (X2 a l n) (Y2 a (offset b a l) n) := by
-    rw [← @f_lzero k b l]
-    rw [f_comp]
-    have h_m := @h_maps_to (offset b a l) k a n
-    apply Set.MapsTo.comp
-    · apply h_maps_to
-    · apply Set.MapsTo.comp
-      · apply (f_maps_to p)
-      · apply g_maps_to
+  exact Set.InvOn.bijOn (f_inv_on p) (f_maps_to' p) (f_inv_maps_to' p)
 
-  have hf' : Set.MapsTo (f_inv (offset b a l) a l) (Y2 a (offset b a l) n) (X2 a l n) := by
-    rw [f_comp']
-    apply Set.MapsTo.comp
-    · apply Set.MapsTo.comp
-      · apply g_maps_to'
-      · apply f_inv_maps_to p
-    · apply  h_maps_to'
 
-  exact Set.InvOn.bijOn (f_inv_on p) hf hf'
+def X3 (as ls : Vector Int (k+1)) (n : Int)
+(C: Vector Int (k+1) → Prop)
+: Set (Vector Int (k+1)) :=
+  {xs : Vector Int (k+1) |
+    xs.head < ls.head + n ∧
+    (∀ i: Fin (k+1), ls.get i ≤ xs.get i) ∧
+    (∀ i: Fin (k+1), ↑i<k →
+      (0 < as.last → upToProd as ls xs (i+1)  < as.get i) ∧
+      (as.last < 0 → as.get i < upToProd as ls xs (i+1))
+    )
+    ∧ C xs
+  }
+
+def Y3 (as ls: Vector Int (k+1)) (off n: Int)
+(C: Vector Int (k+1) → Prop)
+: Set Int :=
+  {x : Int |
+    base off as x k % as.last = 0 ∧
+    (0<as.last → 0 ≤ x-off ∧ x-off < as.head*n) ∧
+    (as.last<0 → as.head*n < x-off ∧ x-off ≤ 0)
+    ∧ C (f_inv off as ls x)
+  }
+
+lemma implies_eq_and{a b: Prop}: ((a → b) ∧ a) = (b ∧ a) := by
+  apply Eq.propIntro
+  tauto
+  tauto
+
+lemma set_implies' {a b: α → Prop} {s : α}: {s: α | b s ∧ a s} = {s: α | (a s → b s) ∧ a s} := by
+  conv =>
+    -- rhs
+    -- rw [setOf]
+    -- arg 2
+    pattern (_ → _) ∧ _
+    rw [implies_eq_and]
+
+
+lemma X3_subset_X2 (a l: Vector Int (k+1)) (n: Int) (C: Vector Int (k+1) → Prop):
+  X3 a l n C ⊆ X2 a l n := by
+  -- rw [Set.inter_comm, Set.left_eq_inter]
+  intro xs
+  intro h
+  constructor
+  apply h.left
+  constructor
+  apply h.right.left
+  apply h.right.right.left
+
+lemma Y3_subset_Y2 (a l: Vector Int (k+1)) (n: Int) (C: Vector Int (k+1) → Prop):
+  Y3 a l off n C = Y2 a off n ∩ Y3 a l off n C := by
+  rw [Set.inter_comm, Set.left_eq_inter]
+  intro xs
+  intro h
+  constructor
+  apply h.left
+  constructor
+  apply h.right.left
+  apply h.right.right.left
+
+lemma Y3_subset_Y2' (a l: Vector Int (k+1)) (n: Int) (C: Vector Int (k+1) → Prop):
+  Y3 a l off n C = Y2 a off n ∩ {x : Int | C (f_inv off a l x)}  := by
+  rw [Y3]
+  conv =>
+    lhs
+    pattern _ ∧ _
+    tactic =>
+      nth_rewrite 2 [← and_assoc]
+      nth_rewrite 1 [← and_assoc]
+  rw [Set.setOf_and]
+  rw [Y2]
+
+lemma X3_subset_X3' (a l: Vector Int (k+1)) (n: Int) (C: Vector Int (k+1) → Prop):
+  X3 a l n C = X2 a l n ∩ {x : Vector Int (k+1) | C x}  := by
+  rw [X3]
+  conv =>
+    lhs
+    pattern _ ∧ _
+    tactic =>
+      nth_rewrite 2 [← and_assoc]
+      nth_rewrite 1 [← and_assoc]
+  rw [Set.setOf_and]
+  rw [X2]
+
+
+
+lemma cond_image  {α : Type u_1} {β : Type u_2} {f : α → β} {f_inv : β → α} {s : Set α} {t : Set β} {p : α → Prop}
+  (inv: Set.InvOn f_inv f s t) (bij: Set.BijOn f s t):
+  f '' ((s ∩ {x : α | p x})) = t ∩ {y : β | p (f_inv y)} := by
+  apply Set.Subset.antisymm
+  case h₁ =>
+    intro y yinIm
+    match yinIm with
+    | ⟨x, xin, h⟩ =>
+    have xinS: x ∈ s := by
+      apply Set.mem_of_mem_inter_left xin
+    have xinPx: x ∈ {x | p x} := by
+      apply Set.mem_of_mem_inter_right xin
+    apply Set.mem_inter
+    have h1 := Set.BijOn.image_eq bij
+    rw [← h, ← h1]
+    use x
+    apply Set.mem_setOf.mpr
+    have eq: f_inv y = x := by
+      rw [← h]
+      apply Set.RightInvOn.eq inv.left xinS
+    rw [eq]
+    apply Set.mem_setOf.mp xinPx
+  case h₂ =>
+    intro y yinInter
+    match yinInter with
+    | ⟨yinT, yinP⟩ =>
+    use (f_inv y)
+    constructor
+    apply Set.mem_inter
+    have h1 := Set.BijOn.image_eq (Set.BijOn.symm inv.symm bij)
+    rw [← h1]
+    use y
+    apply yinP
+    apply Set.RightInvOn.eq inv.right yinT
+
+theorem f_bij_on' {l a: Vector Int (k+1)} (p: Props2 a n) (C: Vector Int (k+1) → Prop):
+  Set.BijOn (f b a ls_zero) (X3 a l n C) ((f b a ls_zero) '' (X3 a l n C)) := by
+  apply Set.BijOn.subset_left (f_bij_on p) (X3_subset_X2 a l n C)
