QuantifierLean/Lemmas2_1.lean
@@ -1,0 +1,9 @@
+
+import Mathlib.Tactic
+import QuantifierLean.Definitions2
+import QuantifierLean.Lemmas2
+
+import Mathlib.Data.Vector.Snoc
+import Mathlib.Logic.Basic
+
+open Mathlib
